Checkpoint

src/AsyncFSDiskSec.v
@@ -87,13 +87,13 @@ Definition tree_equivalent_for tag tree1 tree2:=
   filter tag tree1 = filter tag tree2.
 
 
-Fixpoint only_reads_permitted {T} pr (p: prog T) d:=
+Fixpoint only_reads_permitted {T} pr (p: prog T) d bm hm:=
   match p with
   | Read n => forall vs, d n = Some vs -> can_access pr (fst (fst vs))
-  | Bind p1 p2 => only_reads_permitted pr p1 d /\
-                 forall tr bm hm d' bm' hm' r tr',
+  | Bind p1 p2 => only_reads_permitted pr p1 d bm hm /\
+                 forall tr d' bm' hm' r tr',
                    exec pr tr d bm hm p1 (Finished d' bm' hm' r) tr' ->
-                   only_reads_permitted pr (p2 r) d'
+                   only_reads_permitted pr (p2 r) d' bm' hm'
   | _ => True
   end.
 
@@ -102,7 +102,7 @@ Theorem exec_equivalent:
   forall T (p: prog T) pr tr d1 d2 bm hm d1' bm' hm' tr' (r: T),
     exec pr tr d1 bm hm p (Finished d1' bm' hm' r) tr' ->
     (forall tag, can_access pr tag -> equivalent_for tag d1 d2) ->
-    only_reads_permitted pr p d1 ->
+    only_reads_permitted pr p d1 bm hm ->
     exists d2', exec pr tr d2 bm hm p (Finished d2' bm' hm' r) tr' /\
      (forall tag, can_access pr tag -> equivalent_for tag d1' d2').
 Proof.
@@ -195,7 +195,7 @@ Theorem exec_fbasic_equivalent:
   forall T (p: fbasic T) pr tr d1 d2 bm hm d1' bm' hm' tr' fsxp mscs mscs' (r: T),
     exec_fbasic pr tr d1 bm hm fsxp mscs p (Finished d1' bm' hm' r) mscs' tr' ->
     (forall tag, can_access pr tag -> equivalent_for tag d1 d2) ->
-    only_reads_permitted pr (fbasic_to_prog fsxp mscs p) d1 ->
+    only_reads_permitted pr (fbasic_to_prog fsxp mscs p) d1 bm hm ->
     exists d2', exec_fbasic pr tr d2 bm hm fsxp mscs p (Finished d2' bm' hm' r) mscs' tr' /\
      (forall tag, can_access pr tag -> equivalent_for tag d1' d2').
 Proof.
@@ -214,7 +214,7 @@ Theorem fbasic_return :
    mscs mscs1' fsxp d1 bm hm d1' bm1' hm1' tr1 tr1' d2 (r: T),
    (forall tag, can_access pr tag -> equivalent_for tag d1 d2) ->                     
    exec_fbasic pr tr1 d1 bm hm fsxp mscs p (Finished d1' bm1' hm1' r) mscs1' tr1' ->
-   only_reads_permitted pr (fbasic_to_prog fsxp mscs p) d1 ->
+   only_reads_permitted pr (fbasic_to_prog fsxp mscs p) d1 bm hm ->
   exists d2',
     exec_fbasic pr tr1 d2 bm hm fsxp mscs p (Finished d2' bm1' hm1' r) mscs1' tr1' /\
     (forall tag, can_access pr tag -> equivalent_for tag d1' d2').
@@ -237,7 +237,7 @@ Theorem exec_fprog_equivalent:
   forall T (p: fprog T) pr tr d1 d2 bm hm d1' bm' hm' tr' fsxp mscs mscs' (r: T),
     fexec pr tr d1 bm hm fsxp mscs p (Finished d1' bm' hm' r) mscs' tr' ->
     (forall tag, can_access pr tag -> equivalent_for tag d1 d2) ->
-    only_reads_permitted pr (fprog_to_prog fsxp mscs p) d1 ->
+    only_reads_permitted pr (fprog_to_prog fsxp mscs p) d1 bm hm ->
     exists d2', fexec pr tr d2 bm hm fsxp mscs p (Finished d2' bm' hm' r) mscs' tr' /\
      (forall tag, can_access pr tag -> equivalent_for tag d1' d2').
 Proof.
@@ -260,3 +260,761 @@ Proof.
   econstructor; eauto.
   inversion H19.
 Qed.
+
+
+ Lemma authenticate_post:
+    forall Fr Fm Ftop pathname f dx ds sm tree mscs fsxp ilist frees d bm hm pr inum tr d' bm' hm' tr' (rx: (BFILE.memstate * (bool * unit))),
+      
+      (Fr * [[ sync_invariant Fr ]] *
+       LOG.rep (FSXPLog fsxp) (SB.rep fsxp) (LOG.ActiveTxn ds dx) (MSLL mscs) sm bm hm *
+       [[[ dx ::: (Fm * rep fsxp Ftop tree ilist frees mscs sm) ]]] *
+       [[ find_subtree pathname tree = Some (TreeFile inum f) ]])%pred d ->
+  
+  exec pr tr d bm hm (authenticate fsxp inum mscs)
+       (Finished d' bm' hm' rx) tr' ->
+  let mscs':= fst rx in
+  let r := fst (snd rx) in
+  (Fr * [[ sync_invariant Fr ]] *
+   LOG.rep (FSXPLog fsxp) (SB.rep fsxp) (LOG.ActiveTxn ds dx) (MSLL mscs') sm bm' hm' *
+   [[[ dx ::: (Fm * rep fsxp Ftop tree ilist frees mscs' sm) ]]] *
+   [[ MSAlloc mscs' = MSAlloc mscs ]] *
+   [[ MSCache mscs' = MSCache mscs ]] *
+   [[ MSAllocC mscs' = MSAllocC mscs ]] *
+   [[ MSIAllocC mscs' = MSIAllocC mscs ]] *
+   [[ MSDBlocks mscs' = MSDBlocks mscs ]] *
+   (([[ r = true ]] * [[ can_access pr (DFOwner f) ]]) \/
+    ([[ r = false ]] * [[ ~can_access pr (DFOwner f) ]])))%pred d'.
+  Proof.
+    unfold sys_rep, corr2; intros.
+    pose proof (@authenticate_ok fsxp inum mscs pr) as Hok.
+    specialize (Hok _ (fun r => Ret r)).
+    unfold corr2 in *.
+    edestruct Hok with (d:= d).
+    pred_apply; cancel.
+    eauto.
+    eauto.
+    inv_exec_perm.
+    simpl in *.
+    destruct_lift H1.
+    eassign (fun d0 bm0 hm0 (rx: (BFILE.memstate * (bool * unit))) =>
+               let a:= fst rx in
+               let a1:= fst (snd rx) in
+               (Fr
+         ✶ LOG.rep (FSXPLog fsxp) (SB.rep fsxp) (LOG.ActiveTxn ds dx) (MSLL a) sm bm0 hm0 *
+   [[[ dx ::: (Fm * rep fsxp Ftop tree ilist (frees_1, frees_2) a sm) ]]] *
+   [[ MSAlloc a = MSAlloc mscs ]] *
+   [[ MSCache a = MSCache mscs ]] *
+   [[ MSAllocC a = MSAllocC mscs ]] *
+   [[ MSIAllocC a = MSIAllocC mscs ]] *
+   [[ MSDBlocks a = MSDBlocks mscs ]] *
+   (([[ a1 = true ]] * [[ can_access pr (DFOwner f) ]]) \/
+    ([[ a1 = false ]] * [[ ~can_access pr (DFOwner f) ]])))%pred d0).
+    left; repeat eexists; simpl in *; eauto.
+    pred_apply; cancel.
+    or_l; cancel.
+    or_r; cancel.
+    unfold permission_secure; intros.
+    inv_exec_perm.
+    cleanup; auto.
+    unfold trace_secure; eauto.
+    eassign (fun (_:block_mem) (_:hashmap) (_:rawdisk) => True).
+    intros; simpl; auto.
+    econstructor; eauto.
+    econstructor.
+    simpl in *.
+    destruct rx, p.
+    intuition; cleanup.
+    sigT_eq; eauto.
+    destruct_lift H; subst.
+    pred_apply; cancel.
+    or_l; cancel.
+    or_r; cancel.
+    inversion H1.
+  Qed.
+
+
+
+  Lemma LOG_begin_post:
+    forall Fr ds sm mscs fsxp d bm hm pr tr d' bm' hm' tr' (rx: LOG.mstate * cachestate),
+      
+  (Fr * [[ sync_invariant Fr ]] *
+   LOG.rep (FSXPLog fsxp) (SB.rep fsxp) (LOG.NoTxn ds) (MSLL mscs) sm bm hm)%pred d ->
+  
+  exec pr tr d bm hm (LOG.begin (FSXPLog fsxp) (MSLL mscs))
+       (Finished d' bm' hm' rx) tr' ->
+  (Fr * [[ sync_invariant Fr ]] *
+   LOG.rep (FSXPLog fsxp) (SB.rep fsxp) (LOG.ActiveTxn ds ds!!) rx sm bm' hm' *
+  [[ LOG.readOnly (MSLL mscs) rx ]])%pred d'.
+  Proof.
+     unfold sys_rep, corr2; intros.
+    pose proof (@LOG.begin_ok (FSXPLog fsxp) (MSLL mscs) pr) as Hok.
+    specialize (Hok _ (fun r => Ret r)).
+    unfold corr2 in *.
+    edestruct Hok with (d:= d).
+    pred_apply; cancel.
+    eauto.
+    eauto.
+    inv_exec_perm.
+    simpl in *.
+    destruct_lift H1.
+    eassign (fun d0 bm0 hm0 (rx: LOG.mstate * cachestate) =>
+               let a:= fst rx in
+               let b:= snd rx in
+               (Fr
+        ✶ LOG.rep (FSXPLog fsxp) (SB.rep fsxp) (LOG.ActiveTxn ds ds !!) 
+            (a, b) sm bm0 hm0 * [[ LOG.readOnly (MSLL mscs) (a, b) ]] )%pred d0).
+    left; repeat eexists; simpl in *; eauto.
+    pred_apply; cancel.
+    unfold permission_secure; intros.
+    inv_exec_perm.
+    cleanup; auto.
+    unfold trace_secure; eauto.
+    eassign (fun (_:block_mem) (_:hashmap) (_:rawdisk) => True).
+    intros; simpl; auto.
+    econstructor; eauto.
+    econstructor.
+    simpl in *.
+    destruct rx.
+    intuition; cleanup.
+    sigT_eq; eauto.
+    destruct_lift H; subst.
+    pred_apply; cancel.
+    inversion H1.
+  Qed.
+
+
+Require Import FMapAVL.
+Require Import FMapFacts.
+Import AddrMap.
+Import Map MapFacts.
+
+Lemma maybe_evict_post:
+    forall Fr d dx cs bm hm pr tr d' bm' hm' tr' cs',
+      (Fr * [[ sync_invariant Fr ]] * PermCacheDef.rep cs dx bm)%pred d ->
+      exec pr tr d bm hm (maybe_evict cs)
+           (Finished d' bm' hm' cs') tr' ->
+      (Fr * [[ sync_invariant Fr ]] *
+       PermCacheDef.rep cs' dx bm' *
+      [[ forall a, find a (CSMap cs) = None ->
+              find a (CSMap cs') = None ]] *                 
+      [[ cardinal (CSMap cs') < CSMaxCount cs' ]])%pred d'.
+    Proof.
+      intros.
+      pose proof (@maybe_evict_ok cs pr) as Hok.
+      specialize (Hok _ (fun r => Ret r)).
+      unfold corr2 in *.
+      edestruct Hok with (d:= d).
+      pred_apply; cancel.
+      eauto.
+      eauto.
+      inv_exec_perm.
+      simpl in *.
+      destruct_lift H1.
+      eassign (fun d0 (bm0: block_mem) (hm0:hashmap) cs' =>
+                 (Fr * PermCacheDef.rep cs' dx bm0 *
+                 [[ forall a, find a (CSMap cs) = None ->
+                         find a (CSMap cs') = None ]] *                 
+                 [[ cardinal (CSMap cs') < CSMaxCount cs' ]])%pred d0).
+      left; repeat eexists; simpl in *; eauto.
+      pred_apply; cancel.
+      unfold permission_secure; intros.
+      inv_exec_perm.
+      cleanup; auto.
+      unfold trace_secure; eauto.
+      eassign (fun (_:block_mem) (_:hashmap) (_:rawdisk) => True).
+      intros; simpl; auto.
+      econstructor; eauto.
+      econstructor.
+      simpl in *.
+      intuition; cleanup.
+      sigT_eq; eauto.
+      destruct_lift H; subst.
+      pred_apply; cancel.
+      inversion H1.
+    Qed.
+
+Lemma LOG_begin_orp:
+  forall pr a b d bm hm,
+    only_reads_permitted pr (LOG.begin a b) d bm hm.
+Proof.
+  intros.
+  Transparent LOG.begin.
+  unfold LOG.begin; simpl; auto.
+Qed.
+
+Lemma writeback_orp:
+  forall pr a b d bm hm,
+    only_reads_permitted pr (writeback a b) d bm hm.
+Proof.
+  unfold writeback; simpl; intros.
+  destruct (MapUtils.AddrMap.Map.find a (CSMap b)); simpl; auto.
+  destruct p; simpl; auto.
+  destruct b0; simpl; auto.
+Qed.
+
+Hint Resolve LOG_begin_orp writeback_orp.
+
+Lemma maybe_evict_orp:
+  forall pr a d bm hm,
+    only_reads_permitted pr (maybe_evict a) d bm hm.
+Proof.
+  unfold maybe_evict; simpl; intros.
+  destruct (lt_dec (CSCount a) (CSMaxCount a)); simpl; auto.
+  destruct (MapUtils.AddrMap.Map.find 0 (CSMap a)); simpl; auto.
+  intuition; simpl.
+  destruct (MapUtils.AddrMap.Map.find 0 (CSMap r)); simpl; auto.
+  destruct (MapUtils.AddrMap.Map.elements (CSMap a)); simpl; auto.
+  destruct p; simpl; auto.
+  intuition.
+  destruct (MapUtils.AddrMap.Map.find k (CSMap r)); simpl; auto.
+Qed.
+
+Hint Resolve maybe_evict_orp.
+
+Lemma PermCacheDef_read_orp:
+    forall Fr pr a cs dx d bm hm v,
+      (Fr * [[ sync_invariant Fr ]] * PermCacheDef.rep cs dx bm)%pred d ->
+      can_access pr (fst (fst v)) ->
+      dx a = Some v ->
+      only_reads_permitted pr (PermCacheDef.read a cs) d bm hm.
+  Proof.
+    intros; unfold PermCacheDef.read; simpl.
+    destruct (MapUtils.AddrMap.Map.find a (CSMap cs)) eqn:D; simpl; auto.
+    destruct p; simpl; auto.
+    intuition; simpl.   
+    pose proof (maybe_evict_post H H2) as Hspec.
+    destruct_lift Hspec.
+    specialize H8 with (1:=D).
+    unfold PermCacheDef.rep in *.
+    rewrite mem_pred_extract in H4; eauto.
+    unfold cachepred at 2 in H4.
+    rewrite H8 in H4.
+    repeat rewrite sep_star_assoc in H4.
+    apply sep_star_assoc in H4.
+    apply sep_star_assoc in H4.
+    apply sep_star_assoc in H4.
+    eapply ptsto_subset_valid' in H4.
+    simpl in *; cleanup; eauto.
+  Qed.
+
+  
+
+  Lemma getowner_orp:
+    forall pr d bm hm fsxp inum mscs pathname Fr Fm ds sm Ftop tree ilist frees f,
+      (Fr * [[ sync_invariant Fr ]] *
+       LOG.rep (FSXPLog fsxp) (SB.rep fsxp)
+               (LOG.ActiveTxn ds ds !!) (MSLL mscs) sm bm hm *
+       [[[ ds!! ::: (Fm * rep fsxp Ftop tree ilist frees mscs sm)]]] *
+       [[ find_subtree pathname tree = Some (TreeFile inum f) ]])%pred d ->
+      only_reads_permitted pr (getowner fsxp inum mscs) d bm hm.
+  Proof.
+    intros; unfold getowner.
+
+  Lemma BFILE_getowner_orp:
+    forall pr d bm hm fsxp inum mscs pathname Fr Fm ds sm Ftop tree ilist frees f,
+      (Fr * [[ sync_invariant Fr ]] *
+       LOG.rep (FSXPLog fsxp) (SB.rep fsxp)
+               (LOG.ActiveTxn ds ds !!) (MSLL mscs) sm bm hm *
+       [[[ ds!! ::: (Fm * rep fsxp Ftop tree ilist frees mscs sm)]]] *
+       [[ find_subtree pathname tree = Some (TreeFile inum f) ]])%pred d ->
+      only_reads_permitted pr (BFILE.getowner (FSXPLog fsxp) (FSXPInode fsxp) inum mscs) d bm hm.
+  Proof.
+    intros; unfold BFILE.getowner.
+
+
+  Lemma INODE_getowner_orp:
+    forall pr d bm hm fsxp inum mscs pathname Fr Fm ds sm Ftop tree ilist frees f,
+      (Fr * [[ sync_invariant Fr ]] *
+       LOG.rep (FSXPLog fsxp) (SB.rep fsxp)
+               (LOG.ActiveTxn ds ds !!) (MSLL mscs) sm bm hm *
+       [[[ ds!! ::: (Fm * rep fsxp Ftop tree ilist frees mscs sm)]]] *
+       [[ find_subtree pathname tree = Some (TreeFile inum f) ]])%pred d ->
+      only_reads_permitted pr (INODE.getowner (FSXPLog fsxp) (FSXPInode fsxp) inum (MSICache mscs) (MSLL mscs)) d bm hm.
+  Proof.
+    intros; unfold INODE.getowner.
+
+
+
+  Lemma INODE_IRec_get_array_orp:
+    forall pr d bm hm fsxp inum mscs pathname Fr Fm ds sm Ftop tree ilist frees f,
+      (Fr * [[ sync_invariant Fr ]] *
+       LOG.rep (FSXPLog fsxp) (SB.rep fsxp)
+               (LOG.ActiveTxn ds ds !!) (MSLL mscs) sm bm hm *
+       [[[ ds!! ::: (Fm * rep fsxp Ftop tree ilist frees mscs sm)]]] *
+       [[ find_subtree pathname tree = Some (TreeFile inum f) ]])%pred d ->
+      only_reads_permitted pr (INODE.IRec.get_array (FSXPLog fsxp) (FSXPInode fsxp) inum (MSICache mscs) (MSLL mscs)) d bm hm.
+  Proof.
+    intros; unfold INODE.IRec.get_array.
+
+   Lemma INODE_IRec_get_orp:
+    forall pr d bm hm fsxp inum mscs pathname Fr Fm ds sm Ftop tree ilist frees f,
+      (Fr * [[ sync_invariant Fr ]] *
+       LOG.rep (FSXPLog fsxp) (SB.rep fsxp)
+               (LOG.ActiveTxn ds ds !!) (MSLL mscs) sm bm hm *
+       [[[ ds!! ::: (Fm * rep fsxp Ftop tree ilist frees mscs sm)]]] *
+       [[ find_subtree pathname tree = Some (TreeFile inum f) ]])%pred d ->
+      only_reads_permitted pr (INODE.IRec.get (FSXPLog fsxp) (FSXPInode fsxp) inum (MSICache mscs) (MSLL mscs)) d bm hm.
+  Proof.
+    intros; unfold INODE.IRec.get.
+    destruct (INODE.IRec.Cache.find inum (MSICache mscs)) eqn:D;
+    setoid_rewrite D.
+    simpl; auto.
+
+  Lemma INODE_IRec_LRA_get_orp:
+    forall pr d bm hm fsxp inum mscs pathname Fr Fm ds sm Ftop tree ilist frees f,
+      (Fr * [[ sync_invariant Fr ]] *
+       LOG.rep (FSXPLog fsxp) (SB.rep fsxp)
+               (LOG.ActiveTxn ds ds !!) (MSLL mscs) sm bm hm *
+       [[[ ds!! ::: (Fm * rep fsxp Ftop tree ilist frees mscs sm)]]] *
+       [[ find_subtree pathname tree = Some (TreeFile inum f) ]])%pred d ->
+      INODE.IRec.Cache.find inum (MSICache mscs) = None ->
+      only_reads_permitted pr (INODE.IRec.LRA.get (FSXPLog fsxp) (FSXPInode fsxp) inum (MSLL mscs)) d bm hm.
+  Proof.
+    intros; unfold INODE.IRec.LRA.get.
+
+ Lemma LOG_read_array_orp:
+    forall pr d bm hm fsxp inum mscs pathname Fr Fm ds sm Ftop tree ilist frees f,
+      (Fr * [[ sync_invariant Fr ]] *
+       LOG.rep (FSXPLog fsxp) (SB.rep fsxp)
+               (LOG.ActiveTxn ds ds !!) (MSLL mscs) sm bm hm *
+       [[[ ds!! ::: (Fm * rep fsxp Ftop tree ilist frees mscs sm)]]] *
+       [[ find_subtree pathname tree = Some (TreeFile inum f) ]])%pred d ->
+      INODE.IRec.Cache.find inum (MSICache mscs) = None ->
+      only_reads_permitted pr (LOG.read_array (FSXPLog fsxp) (INODE.IRecSig.RAStart (FSXPInode fsxp))
+       (inum / INODE.IRecSig.items_per_val) (MSLL mscs)) d bm hm.
+  Proof.
+    intros; unfold LOG.read_array.
+    simpl; intuition.
+    destruct_lift H.
+    denote LOG.rep as Hx.
+    unfold LOG.rep, LOG.rep_inner, GLog.rep, MLog.rep, MLog.synced_rep in Hx. destruct_lift Hx.
+    assert (INODE.IRecSig.RAStart (FSXPInode fsxp) +
+            inum / INODE.IRecSig.items_per_val < length dummy1).
+    destruct fsxp; simpl in *.
+
+    denote rep as Hx.
+    unfold rep, FSXPBlockAlloc in Hx; destruct_lift Hx; simpl in *.
+    denote BFILE.rep as Hx. unfold BFILE.rep in Hx.
+    destruct_lift Hx.
+    denote INODE.rep as Hx. unfold INODE.rep, INODE.IRec.rep, INODE.IRec.LRA.rep in Hx.
+    destruct_lift Hx.
+    destruct mscs, MSLL, m, MSGLog; simpl in *.
+    unfold LogReplay.map_replay in *.
+    unfold LogReplay.map_valid in *.
+    Search dummy1.
+    Search MSMLog.
+    unfold PermDiskLog.rep, rep_common,
+    PermDiskLogPadded.rep, rep_inner, rep_contents in *.
+    Search dummy0.
+    Search MSTxns.
+    Search GLog.effective.
+    unfold LOG.MSLL; simpl.
+    destruct ms_1; simpl in *.
+    eapply GLog_read_orp.
+    pred_apply; cancel.
+    
+
+    Lemma MLog_read_orp:
+    forall v pr d bm hm Fr a log ds Ftop MSMLog ms_2 (MSTxns: list input_contents) dummy dx ,
+      (Fr * [[ sync_invariant Fr ]] *
+      PermCacheDef.rep ms_2 dx bm)%pred d ->
+      dx (DataStart log + a) = Some v ->
+      can_access pr (fst (fst v)) ->
+      (Ftop * MLog.rep log (MLog.Synced dummy (nthd (length (snd ds) - length MSTxns) ds)) MSMLog bm hm)%pred dx ->
+      only_reads_permitted pr  (MLog.read log a (MLog.mk_memstate MSMLog ms_2)) d bm hm.
+  Proof.
+    intros; unfold MLog.read.
+    destruct (MapUtils.AddrMap.Map.find a (MLog.MSInLog (MLog.mk_memstate MSMLog ms_2))) eqn:D.
+    simpl; auto.
+    simpl; intuition.
+    eapply PermCacheDef_read_orp; eauto.
+  Qed.
+    
+    Lemma GLog_read_orp:
+    forall v pr d bm hm Fr a log dx MSGLog ms_2 ds Ftop,
+      (Fr * [[ sync_invariant Fr ]] *
+       PermCacheDef.rep ms_2 dx bm)%pred d ->
+      dx (DataStart log + a) = Some v ->
+      can_access pr (fst (fst v)) ->
+     (Ftop ✶ GLog.rep log (GLog.Cached ds) MSGLog bm hm)%pred dx ->
+      only_reads_permitted pr (GLog.read log a (MSGLog, ms_2)) d bm hm.
+  Proof.
+    intros; unfold GLog.read.
+    destruct (MapUtils.AddrMap.Map.find a (GLog.MSVMap (fst (MSGLog, ms_2)))) eqn:D.
+    simpl; auto.
+    simpl; intuition.
+    denote GLog.rep as Hx.
+    unfold GLog.rep in Hx; destruct_lift Hx.
+    destruct MSGLog; simpl in *.
+    unfold GLog.MSLL; simpl.
+    eapply MLog_read_orp; eauto.
+  Qed.
+
+
+ Lemma LOG_read_orp:
+    forall v pr d bm hm log a Fr ds sm ms Ftop,
+      (Fr * [[ sync_invariant Fr ]] *
+       LOG.rep log Ftop (LOG.ActiveTxn ds ds !!) ms sm bm hm)%pred d ->
+      d (DataStart log + a) = Some v ->
+      can_access pr (fst (fst v)) ->
+      only_reads_permitted pr (LOG.read log a ms) d bm hm.
+  Proof.
+    intros; unfold LOG.read.
+    destruct (MapUtils.AddrMap.Map.find a (LOG.MSTxn (fst ms))) eqn:D.
+    simpl; auto.
+    simpl; auto; intuition.
+    denote LOG.rep as Hx.
+    unfold LOG.rep in Hx. destruct_lift Hx.
+    unfold LOG.MSLL; simpl.
+    destruct ms_1; simpl in *.
+    eapply GLog_read_orp.
+    pred_apply; cancel.
+    
+  
+  
+    Lemma read_array_orp:
+    forall pr d bm hm fsxp inum mscs pathname Fr Fm ds sm Ftop tree ilist frees f,
+      (Fr * [[ sync_invariant Fr ]] *
+       LOG.rep (FSXPLog fsxp) (SB.rep fsxp)
+               (LOG.ActiveTxn ds ds !!) (MSLL mscs) sm bm hm *
+       [[[ ds!! ::: (Fm * rep fsxp Ftop tree ilist frees mscs sm)]]] *
+       [[ find_subtree pathname tree = Some (TreeFile inum f) ]])%pred d ->
+      INODE.IRec.Cache.find inum (MSICache mscs) = None ->
+      MapUtils.AddrMap.Map.find
+        (INODE.IRecSig.RAStart (FSXPInode fsxp) +
+         inum / INODE.IRecSig.items_per_val) (LOG.MSTxn (fst (MSLL mscs))) =
+      None ->
+      MapUtils.AddrMap.Map.find
+        (INODE.IRecSig.RAStart (FSXPInode fsxp) +
+         inum / INODE.IRecSig.items_per_val)
+        (GLog.MSVMap (fst (LOG.MSLL (MSLL mscs)))) = None ->
+      MapUtils.AddrMap.Map.find
+        (INODE.IRecSig.RAStart (FSXPInode fsxp) +
+         inum / INODE.IRecSig.items_per_val)
+        (MLog.MSInLog (GLog.MSLL (LOG.MSLL (MSLL mscs)))) = None ->
+      only_reads_permitted pr (read_array (DataStart (FSXPLog fsxp))
+                                (INODE.IRecSig.RAStart (FSXPInode fsxp) +
+                                  inum / INODE.IRecSig.items_per_val)
+                                   (MLog.MSCache (GLog.MSLL (LOG.MSLL (MSLL mscs))))) d bm hm.
+  Proof.
+    intros; unfold read_array.
+    simpl; intuition.
+    unfold LOG.rep in *.
+    destruct_lift H.
+    eapply PermCacheDef_read_orp.
+    pred_apply; cancel.
+
+    unfold LOG.rep_inner in *.
+    destruct_lift H8.
+    unfold GLog.rep in *.
+    destruct_lift H4.
+    unfold MLog.rep in *.
+    destruct_lift H4.
+    unfold PermDiskLog.rep in *.
+    destruct_lift H4.
+
+
+
+
+
+
+
+
+
+
+
+
+
+
+
+    (*******************************************************)
+
+ Lemma LOG_read_orp:
+    forall pr d bm hm fsxp inum mscs pathname Fr Fm ds sm Ftop tree ilist frees f,
+      (Fr * [[ sync_invariant Fr ]] *
+       LOG.rep (FSXPLog fsxp) (SB.rep fsxp)
+               (LOG.ActiveTxn ds ds !!) (MSLL mscs) sm bm hm *
+       [[[ ds!! ::: (Fm * rep fsxp Ftop tree ilist frees mscs sm)]]] *
+       [[ find_subtree pathname tree = Some (TreeFile inum f) ]])%pred d ->
+      INODE.IRec.Cache.find inum (MSICache mscs) = None ->
+      only_reads_permitted pr (LOG.read (FSXPLog fsxp)
+       (INODE.IRecSig.RAStart (FSXPInode fsxp) +
+        inum / INODE.IRecSig.items_per_val) (MSLL mscs)) d bm hm.
+  Proof.
+    intros; unfold LOG.read.
+    destruct (MapUtils.AddrMap.Map.find
+        (INODE.IRecSig.RAStart (FSXPInode fsxp) +
+         inum / INODE.IRecSig.items_per_val) (LOG.MSTxn (fst (MSLL mscs)))) eqn:D.
+    simpl; auto.
+
+
+
+    Lemma GLog_read_orp:
+    forall pr d bm hm fsxp inum mscs pathname Fr Fm ds sm Ftop tree ilist frees f,
+      (Fr * [[ sync_invariant Fr ]] *
+       LOG.rep (FSXPLog fsxp) (SB.rep fsxp)
+               (LOG.ActiveTxn ds ds !!) (MSLL mscs) sm bm hm *
+       [[[ ds!! ::: (Fm * rep fsxp Ftop tree ilist frees mscs sm)]]] *
+       [[ find_subtree pathname tree = Some (TreeFile inum f) ]])%pred d ->
+      INODE.IRec.Cache.find inum (MSICache mscs) = None ->
+      MapUtils.AddrMap.Map.find
+        (INODE.IRecSig.RAStart (FSXPInode fsxp) +
+         inum / INODE.IRecSig.items_per_val) (LOG.MSTxn (fst (MSLL mscs))) =
+      None ->
+      only_reads_permitted pr (GLog.read (FSXPLog fsxp)
+                               (INODE.IRecSig.RAStart (FSXPInode fsxp) +
+                                inum / INODE.IRecSig.items_per_val)
+                                 (LOG.MSLL (MSLL mscs))) d bm hm.
+  Proof.
+    intros; unfold GLog.read.
+    destruct (MapUtils.AddrMap.Map.find
+        (INODE.IRecSig.RAStart (FSXPInode fsxp) +
+         inum / INODE.IRecSig.items_per_val)
+        (GLog.MSVMap (fst (LOG.MSLL (MSLL mscs))))) eqn:D.
+    simpl; auto.
+
+
+    Lemma MLog_read_orp:
+    forall pr d bm hm fsxp inum mscs pathname Fr Fm ds sm Ftop tree ilist frees f,
+      (Fr * [[ sync_invariant Fr ]] *
+       LOG.rep (FSXPLog fsxp) (SB.rep fsxp)
+               (LOG.ActiveTxn ds ds !!) (MSLL mscs) sm bm hm *
+       [[[ ds!! ::: (Fm * rep fsxp Ftop tree ilist frees mscs sm)]]] *
+       [[ find_subtree pathname tree = Some (TreeFile inum f) ]])%pred d ->
+      INODE.IRec.Cache.find inum (MSICache mscs) = None ->
+      MapUtils.AddrMap.Map.find
+        (INODE.IRecSig.RAStart (FSXPInode fsxp) +
+         inum / INODE.IRecSig.items_per_val) (LOG.MSTxn (fst (MSLL mscs))) =
+      None ->
+      MapUtils.AddrMap.Map.find
+        (INODE.IRecSig.RAStart (FSXPInode fsxp) +
+         inum / INODE.IRecSig.items_per_val)
+        (GLog.MSVMap (fst (LOG.MSLL (MSLL mscs)))) = None ->
+      only_reads_permitted pr (MLog.read (FSXPLog fsxp)
+                                (INODE.IRecSig.RAStart (FSXPInode fsxp) +
+                                  inum / INODE.IRecSig.items_per_val)
+                                   (GLog.MSLL (LOG.MSLL (MSLL mscs)))) d bm hm.
+  Proof.
+    intros; unfold MLog.read.
+    destruct (MapUtils.AddrMap.Map.find
+        (INODE.IRecSig.RAStart (FSXPInode fsxp) +
+         inum / INODE.IRecSig.items_per_val)
+        (MLog.MSInLog (GLog.MSLL (LOG.MSLL (MSLL mscs))))) eqn:D.
+    simpl; auto.
+
+    Lemma read_array_orp:
+    forall pr d bm hm fsxp inum mscs pathname Fr Fm ds sm Ftop tree ilist frees f,
+      (Fr * [[ sync_invariant Fr ]] *
+       LOG.rep (FSXPLog fsxp) (SB.rep fsxp)
+               (LOG.ActiveTxn ds ds !!) (MSLL mscs) sm bm hm *
+       [[[ ds!! ::: (Fm * rep fsxp Ftop tree ilist frees mscs sm)]]] *
+       [[ find_subtree pathname tree = Some (TreeFile inum f) ]])%pred d ->
+      INODE.IRec.Cache.find inum (MSICache mscs) = None ->
+      MapUtils.AddrMap.Map.find
+        (INODE.IRecSig.RAStart (FSXPInode fsxp) +
+         inum / INODE.IRecSig.items_per_val) (LOG.MSTxn (fst (MSLL mscs))) =
+      None ->
+      MapUtils.AddrMap.Map.find
+        (INODE.IRecSig.RAStart (FSXPInode fsxp) +
+         inum / INODE.IRecSig.items_per_val)
+        (GLog.MSVMap (fst (LOG.MSLL (MSLL mscs)))) = None ->
+      MapUtils.AddrMap.Map.find
+        (INODE.IRecSig.RAStart (FSXPInode fsxp) +
+         inum / INODE.IRecSig.items_per_val)
+        (MLog.MSInLog (GLog.MSLL (LOG.MSLL (MSLL mscs)))) = None ->
+      only_reads_permitted pr (read_array (DataStart (FSXPLog fsxp))
+                                (INODE.IRecSig.RAStart (FSXPInode fsxp) +
+                                  inum / INODE.IRecSig.items_per_val)
+                                   (MLog.MSCache (GLog.MSLL (LOG.MSLL (MSLL mscs))))) d bm hm.
+  Proof.
+    intros; unfold read_array.
+    simpl; intuition.
+    unfold LOG.rep in *.
+    destruct_lift H.
+    eapply PermCacheDef_read_orp.
+    pred_apply; cancel.
+
+    unfold LOG.rep_inner in *.
+    destruct_lift H8.
+    unfold GLog.rep in *.
+    destruct_lift H4.
+    unfold MLog.rep in *.
+    destruct_lift H4.
+    unfold PermDiskLog.rep in *.
+    destruct_lift H4.
+
+  Lemma authenticate_orp:
+    forall pr d bm hm fsxp inum mscs pathname Fr Fm ds sm Ftop tree ilist frees f,
+      (Fr * [[ sync_invariant Fr ]] *
+       LOG.rep (FSXPLog fsxp) (SB.rep fsxp)
+               (LOG.ActiveTxn ds ds !!) (MSLL mscs) sm bm hm *
+       [[[ ds!! ::: (Fm * rep fsxp Ftop tree ilist frees mscs sm)]]] *
+       [[ find_subtree pathname tree = Some (TreeFile inum f) ]])%pred d ->
+      only_reads_permitted pr (authenticate fsxp inum mscs) d bm hm.
+  Proof.
+    intros; unfold authenticate.
+    
+    simpl; auto.
+    intuition; simpl.
+    unfold rep, BFILE.rep in *.
+
+Lemma read_fblock_orp:
+  forall pathname f pr off vs inum Fd
+    Fr1 Fm1 Ftop1 ds1 sm1 tree1 mscs1 fsxp1 ilist1 frees1 d bm1 hm1,
+  (Fr1 * [[ sync_invariant Fr1 ]] *
+     LOG.rep (FSXPLog fsxp1) (SB.rep fsxp1) (LOG.NoTxn ds1) (MSLL mscs1) sm1 bm1 hm1 *
+      [[[ ds1!! ::: (Fm1 * rep fsxp1 Ftop1 tree1 ilist1 frees1 mscs1 sm1)]]] *
+      [[ find_subtree pathname tree1 = Some (TreeFile inum f) ]] *
+      [[[ (DFData f) ::: (Fd * off |-> vs) ]]])%pred d ->
+  only_reads_permitted pr (read_fblock fsxp1 inum off mscs1) d bm1 hm1.
+Proof.  
+  unfold read_fblock; simpl.
+  intuition; simpl; auto.
+
+  assert (A: (Fr1 ✶ ⟦⟦ sync_invariant Fr1 ⟧⟧
+          ✶ LOG.rep (FSXPLog fsxp1) (SB.rep fsxp1) (LOG.NoTxn ds1) 
+          (MSLL mscs1) sm1 bm1 hm1)%pred d).
+    pred_apply; cancel.
+    pose proof (LOG_begin_post _ A H0) as Hspec1.
+
+  (((Fr1 ✶ ⟦⟦ sync_invariant Fr1 ⟧⟧)
+             ✶ LOG.rep (FSXPLog fsxp1) (SB.rep fsxp1)
+                 (LOG.ActiveTxn ds1 ds1 !!) r sm1 bm' hm')
+     ✶ ⟦⟦ LOG.readOnly (MSLL mscs1) r ⟧⟧ *
+   [[[ ds1!! ::: (Fm1 * rep fsxp1 Ftop1 tree1 ilist1 frees1 mscs1 sm1)]]] *
+      [[ find_subtree pathname tree1 = Some (TreeFile inum f) ]])%pred d'
+
+        
+  Lemma MLog_read_orp:
+    forall pr a b c d bm hm dx v Fr,
+      (Fr * [[ sync_invariant Fr ]] *
+       PermCacheDef.rep (MLog.MSCache c) dx bm)%pred d ->
+      can_access pr (fst (fst v)) ->
+      dx (DataStart a + b) = Some v ->
+      only_reads_permitted pr (MLog.read a b c) d bm hm.
+  Proof.
+    intros; unfold MLog.read; simpl; auto.
+    destruct (MapUtils.AddrMap.Map.find b (MLog.MSInLog c)); simpl; auto.
+    intuition; simpl.      
+    eapply PermCacheDef_read_orp; eauto.
+  Qed.
+    
+  Lemma INODE_IRec_get_orp:
+    forall pr a b c x y d bm hm Fr1 sm ds dx k,
+    (Fr1 * [[ sync_invariant Fr1 ]]
+     * LOG.rep a k (LOG.ActiveTxn ds dx) y sm bm hm)%pred d ->
+    only_reads_permitted pr (INODE.IRec.get a b c x y) d bm hm.
+  Proof.
+    intros; unfold INODE.IRec.get; simpl.
+    destruct (INODE.IRec.Cache.find c x) eqn:D;
+    setoid_rewrite D; simpl; auto.
+    intuition; simpl.
+
+    Lemma LOG_read_orp:
+      forall pr a b c d bm hm Fr1 k ds dx sm,
+        ((Fr1 ✶ ⟦⟦ sync_invariant Fr1 ⟧⟧) ✶ LOG.rep a k (LOG.ActiveTxn ds dx) c sm bm hm)%pred d ->
+        only_reads_permitted pr (LOG.read a b c) d bm hm.
+    Proof.
+      intros; unfold LOG.read; simpl.
+      destruct (MapUtils.AddrMap.Map.find b (LOG.MSTxn (fst c))) eqn:D; simpl; auto.
+      intuition; simpl.
+      unfold LOG.rep, LOG.rep_inner in *.
+      destruct_lift H.
+
+      Lemma GLog_read_orp:
+        forall pr a b c d bm hm dx v Fr,
+          (Fr * [[ sync_invariant Fr ]] *
+           PermCacheDef.rep (MLog.MSCache (GLog.MSLL c)) dx bm)%pred d ->
+          can_access pr (fst (fst v)) ->
+          dx (DataStart a + b) = Some v ->
+          only_reads_permitted pr (GLog.read a b c) d bm hm.
+      Proof.
+        intros; unfold GLog.read; simpl.
+        destruct (MapUtils.AddrMap.Map.find b
+                  (GLog.MSVMap (fst c))) eqn:D; simpl; auto.
+        intuition; simpl.
+
+        
+
+      eapply MLog_read_orp; eauto.
+      
+          
+    unfold maybe_evict; simpl.
+    destruct (lt_dec (CSCount (snd r)) (CSMaxCount (snd r))); simpl; eauto.
+    destruct (MapUtils.AddrMap.Map.find 0 (CSMap (snd r))); simpl; auto.
+    intuition; simpl.
+    unfold writeback; simpl.
+    destruct (MapUtils.AddrMap.Map.find 0 (CSMap (snd r))); simpl; auto.
+    destruct p; simpl; auto.
+    destruct b1; simpl; auto.
+    destruct (MapUtils.AddrMap.Map.find 0 (CSMap r0)); simpl; auto.
+    destruct (MapUtils.AddrMap.Map.elements (CSMap (snd r))); simpl; auto.
+    destruct p; auto.
+    unfold evict; simpl; auto.
+    intuition; simpl.
+    unfold writeback; simpl.
+    destruct (MapUtils.AddrMap.Map.find k (CSMap (snd r))); simpl; auto.
+    destruct p; simpl; auto.
+    destruct b1; simpl; auto.
+    destruct (MapUtils.AddrMap.Map.find k (CSMap r0)); simpl; auto.
+
+    admit. (** An Actual Goal **)
+
+  - assert (A: (Fr1 ✶ ⟦⟦ sync_invariant Fr1 ⟧⟧
+          ✶ LOG.rep (FSXPLog fsxp1) (SB.rep fsxp1) (LOG.NoTxn ds1) 
+          (MSLL mscs1) sm1 bm1 hm1)%pred d).
+    pred_apply; cancel.
+    pose proof (LOG_begin_post _ A H0) as Hspec1.
+    assert (A0: (Fr1 * [[ sync_invariant Fr1 ]]
+             * LOG.rep (FSXPLog fsxp1) (SB.rep fsxp1)
+                 (LOG.ActiveTxn ds1 ds1 !!) (MSLL {|
+            BFILE.MSAlloc := MSAlloc mscs1;
+            BFILE.MSLL := r;
+            BFILE.MSAllocC := MSAllocC mscs1;
+            BFILE.MSIAllocC := MSIAllocC mscs1;
+            BFILE.MSICache := MSICache mscs1;
+            BFILE.MSCache := MSCache mscs1;
+            BFILE.MSDBlocks := MSDBlocks mscs1 |}) sm1 bm' hm' *
+       [[[  ds1 !! ::: Fm1 * rep fsxp1 Ftop1 tree1 ilist1 (a, b) mscs1 sm1 ]]] *
+       [[ find_subtree pathname tree1 = Some (TreeFile inum f) ]])%pred d').
+    destruct_lift H.
+    pred_apply; cancel.
+    pose proof (authenticate_post _ A0 H1) as Hspec2.
+    apply sep_star_or_distr in Hspec2.
+    apply pimpl_or_apply in Hspec2.
+    intuition; simpl in *; destruct_lift H2.
+  + intuition; simpl; auto.
+      
+    unfold INODE.IRec.get; simpl; auto.
+    destruct (INODE.IRec.Cache.find inum (MSICache a0)) eqn:D;
+    setoid_rewrite D; simpl; auto.
+    intuition; simpl.
+    unfold LOG.read; simpl; auto.
+    destruct (MapUtils.AddrMap.Map.find
+        (INODE.IRecSig.RAStart (FSXPInode fsxp1) +
+         inum / INODE.IRecSig.items_per_val) (LOG.MSTxn (fst (MSLL a0)))); simpl; auto.
+    unfold GLog.read; simpl; auto.
+    intuition; simpl.
+    destruct (MapUtils.AddrMap.Map.find
+        (INODE.IRecSig.RAStart (FSXPInode fsxp1) +
+         inum / INODE.IRecSig.items_per_val)
+        (GLog.MSVMap (LOG.MSGLog (fst (MSLL a0))))); simpl; auto.
+    intuition; simpl.
+    unfold MLog.read; simpl; auto.
+    destruct (MapUtils.AddrMap.Map.find
+        (INODE.IRecSig.RAStart (FSXPInode fsxp1) +
+         inum / INODE.IRecSig.items_per_val)
+        (GLog.MSMLog (LOG.MSGLog (fst (MSLL a0))))); simpl; auto.
+    intuition; simpl.
+    unfold PermCacheDef.read; simpl; auto.
+    destruct (MapUtils.AddrMap.Map.find
+        (DataStart (FSXPLog fsxp1) +
+         (INODE.IRecSig.RAStart (FSXPInode fsxp1) +
+          inum / INODE.IRecSig.items_per_val)) (CSMap (snd (MSLL a0)))); simpl; auto.
+    destruct p; simpl; auto.
+    intuition; simpl.
+
+    
+      
+    
+    unfold maybe_evict; simpl; auto.
